<?xml version="1.0"?>
<rdf:RDF xmlns="http://localhost:8080/BFiaO/EmergencyAgent#"
     xml:base="http://localhost:8080/BFiaO/EmergencyAgent"
     xmlns:dc="http://purl.org/dc/elements/1.1/"
     xmlns:ns="http://creativecommons.org/ns#"
     xmlns:owl="http://www.w3.org/2002/07/owl#"
     xmlns:rdf="http://www.w3.org/1999/02/22-rdf-syntax-ns#"
     xmlns:xml="http://www.w3.org/XML/1998/namespace"
     xmlns:xsd="http://www.w3.org/2001/XMLSchema#"
     xmlns:rdfs="http://www.w3.org/2000/01/rdf-schema#"
     xmlns:EmergencyAgent="http://localhost:8080/BFiaO/EmergencyAgent#">
    <owl:Ontology rdf:about="http://localhost:8080/BFiaO/EmergencyAgent">
        <ns:license rdf:resource="https://spdx.org/licenses/MIT.html"/>
        <content_license xml:lang="en">The MIT License (MIT)

Copyright (c) 2022 Leopoldo Santos Santos of Strategic Sector

Permission is hereby granted, free of charge, to any person obtaining a copy
of this software and associated documentation files (the &quot;Software&quot;), to deal
in the Software without restriction, including without limitation the rights
to use, copy, modify, merge, publish, distribute, sublicense, and/or sell
copies of the Software, and to permit persons to whom the Software is
furnished to do so, subject to the following conditions:

The above copyright notice and this permission notice shall be included in
all copies or substantial portions of the Software.

THE SOFTWARE IS PROVIDED &quot;AS IS&quot;, WITHOUT WARRANTY OF ANY KIND, EXPRESS OR
IMPLIED, INCLUDING BUT NOT LIMITED TO THE WARRANTIES OF MERCHANTABILITY,
FITNESS FOR A PARTICULAR PURPOSE AND NONINFRINGEMENT. IN NO EVENT SHALL THE
AUTHORS OR COPYRIGHT HOLDERS BE LIABLE FOR ANY CLAIM, DAMAGES OR OTHER
LIABILITY, WHETHER IN AN ACTION OF CONTRACT, TORT OR OTHERWISE, ARISING FROM,
OUT OF OR IN CONNECTION WITH THE SOFTWARE OR THE USE OR OTHER DEALINGS IN
THE SOFTWARE.</content_license>
        <dc:creator xml:lang="en">Leopoldo Santos Santos</dc:creator>
        <rdfs:comment xml:lang="en">This ontology is designed to identify the emergency agents who can act in an emergency situation.</rdfs:comment>
        <rdfs:label>Emergency Agent</rdfs:label>
        <owl:versionInfo xml:lang="en">Version 1.0</owl:versionInfo>
    </owl:Ontology>
    


    <!-- 
    ///////////////////////////////////////////////////////////////////////////////////////
    //
    // Annotation properties
    //
    ///////////////////////////////////////////////////////////////////////////////////////
     -->


    


    <!-- http://creativecommons.org/ns#license -->


    <owl:AnnotationProperty rdf:about="http://creativecommons.org/ns#license"/>
    


    <!-- http://localhost:8080/BFiaO/EmergencyAgent#content_license -->


    <owl:AnnotationProperty rdf:about="http://localhost:8080/BFiaO/EmergencyAgent#content_license"/>
    


    <!-- http://purl.org/dc/elements/1.1/creator -->


    <owl:AnnotationProperty rdf:about="http://purl.org/dc/elements/1.1/creator"/>
    


    <!-- 
    ///////////////////////////////////////////////////////////////////////////////////////
    //
    // Data properties
    //
    ///////////////////////////////////////////////////////////////////////////////////////
     -->


    


    <!-- http://localhost:8080/BFiaO/EmergencyAgent#AgentDeployedGeolocation -->


    <owl:DatatypeProperty rdf:about="http://localhost:8080/BFiaO/EmergencyAgent#AgentDeployedGeolocation">
        <rdfs:comment xml:lang="en">This atribute has the geolacation of the agent.</rdfs:comment>
        <rdfs:isDefinedBy xml:lang="en">This atribute has the geolacation of the agent.</rdfs:isDefinedBy>
        <rdfs:label xml:lang="en">AgentDeployedGeolocation</rdfs:label>
    </owl:DatatypeProperty>
    


    <!-- http://localhost:8080/BFiaO/EmergencyAgent#AgentEndUseTransctionTime -->


    <owl:DatatypeProperty rdf:about="http://localhost:8080/BFiaO/EmergencyAgent#AgentEndUseTransctionTime">
        <rdfs:comment xml:lang="en">It identifies the transaction time for the completion time of use of an artifact by an agent.</rdfs:comment>
        <rdfs:isDefinedBy xml:lang="en">It identifies the transaction time for the completion time of use of an artifact by an agent.</rdfs:isDefinedBy>
        <rdfs:label xml:lang="en">AgentEndUseTransctionTime</rdfs:label>
    </owl:DatatypeProperty>
    


    <!-- http://localhost:8080/BFiaO/EmergencyAgent#AgentEndUseValidTime -->


    <owl:DatatypeProperty rdf:about="http://localhost:8080/BFiaO/EmergencyAgent#AgentEndUseValidTime">
        <rdfs:comment xml:lang="en">It identifies the completion time of use of an artifact by an agent.</rdfs:comment>
        <rdfs:isDefinedBy xml:lang="en">It identifies the completion time of use of an artifact by an agent.</rdfs:isDefinedBy>
        <rdfs:label xml:lang="en">AgentEndUseValidTime</rdfs:label>
    </owl:DatatypeProperty>
    


    <!-- http://localhost:8080/BFiaO/EmergencyAgent#AgentName -->


    <owl:DatatypeProperty rdf:about="http://localhost:8080/BFiaO/EmergencyAgent#AgentName">
        <rdfs:comment xml:lang="en">It identifes the name of an agent.</rdfs:comment>
        <rdfs:isDefinedBy xml:lang="en">It identifes the name of an agent.</rdfs:isDefinedBy>
        <rdfs:label xml:lang="en">AgentName</rdfs:label>
    </owl:DatatypeProperty>
    


    <!-- http://localhost:8080/BFiaO/EmergencyAgent#AgentPhone -->


    <owl:DatatypeProperty rdf:about="http://localhost:8080/BFiaO/EmergencyAgent#AgentPhone">
        <rdfs:comment xml:lang="en">It identifies the phone of the agent.</rdfs:comment>
        <rdfs:isDefinedBy xml:lang="en">It identifies the phone of the agent.</rdfs:isDefinedBy>
        <rdfs:label xml:lang="en">AgentPhone</rdfs:label>
    </owl:DatatypeProperty>
    


    <!-- http://localhost:8080/BFiaO/EmergencyAgent#AgentRank -->


    <owl:DatatypeProperty rdf:about="http://localhost:8080/BFiaO/EmergencyAgent#AgentRank">
        <rdfs:comment xml:lang="en">It identifies the rank of an agent.</rdfs:comment>
        <rdfs:isDefinedBy xml:lang="en">It identifies the rank of an agent.</rdfs:isDefinedBy>
        <rdfs:label xml:lang="en">AgentRank</rdfs:label>
    </owl:DatatypeProperty>
    


    <!-- http://localhost:8080/BFiaO/EmergencyAgent#AgentStartUseTransactionTime -->


    <owl:DatatypeProperty rdf:about="http://localhost:8080/BFiaO/EmergencyAgent#AgentStartUseTransactionTime">
        <rdfs:comment xml:lang="en">It identifies the transaction tiem for start time of use of an artifact by an agent.</rdfs:comment>
        <rdfs:isDefinedBy xml:lang="en">It identifies the transaction tiem for start time of use of an artifact by an agent.</rdfs:isDefinedBy>
        <rdfs:label xml:lang="en">AgentStartUseTransactionTime</rdfs:label>
    </owl:DatatypeProperty>
    


    <!-- http://localhost:8080/BFiaO/EmergencyAgent#AgentStartUseValidTime -->


    <owl:DatatypeProperty rdf:about="http://localhost:8080/BFiaO/EmergencyAgent#AgentStartUseValidTime">
        <rdfs:subPropertyOf rdf:resource="http://www.w3.org/2002/07/owl#topDataProperty"/>
        <rdfs:comment xml:lang="en">It identifies the start time of use of an artifact by an agent.</rdfs:comment>
        <rdfs:isDefinedBy xml:lang="en">It identifies the start time of use of an artifact by an agent.</rdfs:isDefinedBy>
        <rdfs:label xml:lang="en">AgentStartUseValidTime</rdfs:label>
    </owl:DatatypeProperty>
    


    <!-- http://localhost:8080/BFiaO/EmergencyAgent#AgentUnitID -->


    <owl:DatatypeProperty rdf:about="http://localhost:8080/BFiaO/EmergencyAgent#AgentUnitID">
        <rdfs:comment xml:lang="en">It identifies the identification code for the Unit.</rdfs:comment>
        <rdfs:isDefinedBy xml:lang="en">It identifies the identification code for the Unit.</rdfs:isDefinedBy>
        <rdfs:label xml:lang="en">AgentUnitID</rdfs:label>
    </owl:DatatypeProperty>
    


    <!-- 
    ///////////////////////////////////////////////////////////////////////////////////////
    //
    // Classes
    //
    ///////////////////////////////////////////////////////////////////////////////////////
     -->


    


    <!-- http://localhost:8080/BFiaO/EmergencyAgent#armedForcesAgent -->


    <owl:Class rdf:about="http://localhost:8080/BFiaO/EmergencyAgent#armedForcesAgent">
        <rdfs:comment xml:lang="en">It is a person who belongs to Armed Forces.</rdfs:comment>
        <rdfs:isDefinedBy xml:lang="en">It is a person who belongs to Armed Forces.</rdfs:isDefinedBy>
        <rdfs:label xml:lang="en">armedForcesAgent</rdfs:label>
    </owl:Class>
    


    <!-- http://localhost:8080/BFiaO/EmergencyAgent#armedForcesFireExtinguisherPlanePilotAgent -->


    <owl:Class rdf:about="http://localhost:8080/BFiaO/EmergencyAgent#armedForcesFireExtinguisherPlanePilotAgent">
        <rdfs:comment xml:lang="en">A military pilot who has a license to pilot aircraft and specialized in piloting firefighting aircraft.</rdfs:comment>
        <rdfs:isDefinedBy xml:lang="en">A military pilot who has a license to pilot aircraft and specialized in piloting firefighting aircraft.</rdfs:isDefinedBy>
        <rdfs:label xml:lang="en">armedForcesFireExtinguisherPlanePilotAgent</rdfs:label>
    </owl:Class>
    


    <!-- http://localhost:8080/BFiaO/EmergencyAgent#armedForcesHelicopterPilotAgent -->


    <owl:Class rdf:about="http://localhost:8080/BFiaO/EmergencyAgent#armedForcesHelicopterPilotAgent">
        <rdfs:comment xml:lang="en">A military pilot who belong to Armed Forces and has a license to pilot a helicopter.</rdfs:comment>
        <rdfs:isDefinedBy xml:lang="en">A military pilot who belong to Armed Forces and has a license to pilot a helicopter.</rdfs:isDefinedBy>
        <rdfs:label xml:lang="en">armedForcesHelicopterPilotAgent</rdfs:label>
    </owl:Class>
    


    <!-- http://localhost:8080/BFiaO/EmergencyAgent#bRIFAgent -->


    <owl:Class rdf:about="http://localhost:8080/BFiaO/EmergencyAgent#bRIFAgent">
        <rdfs:comment xml:lang="en">It is an agent who belongs to a BRIF.</rdfs:comment>
        <rdfs:isDefinedBy xml:lang="en">It is an agent who belongs to a BRIF.</rdfs:isDefinedBy>
        <rdfs:label xml:lang="en">bRIFAgent</rdfs:label>
    </owl:Class>
    


    <!-- http://localhost:8080/BFiaO/EmergencyAgent#cBRNAgent -->


    <owl:Class rdf:about="http://localhost:8080/BFiaO/EmergencyAgent#cBRNAgent">
        <rdfs:comment xml:lang="en">A CBRN Agent is a person with training in CBRN. CBRN is an acronym for Chemical, Biological, Radiological and Nuclear.</rdfs:comment>
        <rdfs:isDefinedBy xml:lang="en">A CBRN Agent is a person with training in CBRN. CBRN is an acronym for Chemical, Biological, Radiological and Nuclear.</rdfs:isDefinedBy>
        <rdfs:label xml:lang="en">cBRNAgent</rdfs:label>
    </owl:Class>
    


    <!-- http://localhost:8080/BFiaO/EmergencyAgent#cBRNArmedForcesAgent -->


    <owl:Class rdf:about="http://localhost:8080/BFiaO/EmergencyAgent#cBRNArmedForcesAgent">
        <rdfs:comment xml:lang="en">A CBRN Armed Forces Agent is a person with training in CBRN who belongs to Armed Forces. CBRN is an acronym for Chemical, Biological, Radiological and Nuclear.</rdfs:comment>
        <rdfs:isDefinedBy xml:lang="en">A CBRN Armed Forces Agent is a person with training in CBRN who belongs to Armed Forces. CBRN is an acronym for Chemical, Biological, Radiological and Nuclear.</rdfs:isDefinedBy>
        <rdfs:label xml:lang="en">cBRNArmedForcesAgent</rdfs:label>
    </owl:Class>
    


    <!-- http://localhost:8080/BFiaO/EmergencyAgent#cBRNUMEAgent -->


    <owl:Class rdf:about="http://localhost:8080/BFiaO/EmergencyAgent#cBRNUMEAgent">
        <rdfs:comment xml:lang="en">A UME CBRN Agent is a person with training in CBRN who belongs to UME (Emergency Military Unit). CBRN is an acronym for Chemical, Biological, Radiological and Nuclear.</rdfs:comment>
        <rdfs:isDefinedBy xml:lang="en">A UME CBRN Agent is a person with training in CBRN who belongs to UME (Emergency Military Unit). CBRN is an acronym for Chemical, Biological, Radiological and Nuclear.</rdfs:isDefinedBy>
        <rdfs:label xml:lang="en">cBRNUMEAgent</rdfs:label>
    </owl:Class>
    


    <!-- http://localhost:8080/BFiaO/EmergencyAgent#doctorAgent -->


    <owl:Class rdf:about="http://localhost:8080/BFiaO/EmergencyAgent#doctorAgent">
        <rdfs:comment xml:lang="en">A person with a medical degree whose job is to treat people who are ill or hurt and who belongs to any kind of Units working in the Emergency.</rdfs:comment>
        <rdfs:isDefinedBy xml:lang="en">A person with a medical degree whose job is to treat people who are ill or hurt and who belongs to any kind of Units working in the Emergency.</rdfs:isDefinedBy>
        <rdfs:label xml:lang="en">doctorAgent</rdfs:label>
    </owl:Class>
    


    <!-- http://localhost:8080/BFiaO/EmergencyAgent#fireBrigadeAgent -->


    <owl:Class rdf:about="http://localhost:8080/BFiaO/EmergencyAgent#fireBrigadeAgent">
        <rdfs:comment xml:lang="en">A Fire Brigade Agent is a person with training in fire fighting and works in this field.</rdfs:comment>
        <rdfs:isDefinedBy xml:lang="en">A Fire Brigade Agent is a person with training in fire fighting and works in this field.</rdfs:isDefinedBy>
        <rdfs:label xml:lang="en">fireBrigadeAgent</rdfs:label>
    </owl:Class>
    


    <!-- http://localhost:8080/BFiaO/EmergencyAgent#guardiaCivilAgent -->


    <owl:Class rdf:about="http://localhost:8080/BFiaO/EmergencyAgent#guardiaCivilAgent">
        <rdfs:comment xml:lang="en">Is a person who belongs to Guardia Civil, which is a law enforcement force, a gendarmerie corps with a military nature with a permanent vocation for services.</rdfs:comment>
        <rdfs:isDefinedBy xml:lang="en">Is a person who belongs to Guardia Civil, which is a law enforcement force, a gendarmerie corps with a military nature with a permanent vocation for services.</rdfs:isDefinedBy>
        <rdfs:label xml:lang="en">guardiaCivilAgent</rdfs:label>
    </owl:Class>
    


    <!-- http://localhost:8080/BFiaO/EmergencyAgent#healthCareWorkerAgent -->


    <owl:Class rdf:about="http://localhost:8080/BFiaO/EmergencyAgent#healthCareWorkerAgent">
        <rdfs:comment xml:lang="en">A healthcare worker is anyone who works in a healthcare or social care setting, including healthcare students on clinical placement, frontline healthcare workers and other healthcare workers not in direct patient contact.</rdfs:comment>
        <rdfs:isDefinedBy xml:lang="en">A healthcare worker is anyone who works in a healthcare or social care setting, including healthcare students on clinical placement, frontline healthcare workers and other healthcare workers not in direct patient contact.</rdfs:isDefinedBy>
        <rdfs:label xml:lang="en">healthCareWorkerAgent</rdfs:label>
    </owl:Class>
    


    <!-- http://localhost:8080/BFiaO/EmergencyAgent#policeAgent -->


    <owl:Class rdf:about="http://localhost:8080/BFiaO/EmergencyAgent#policeAgent">
        <rdfs:comment xml:lang="en">A person whose job is to enforce laws, investigate crimes, and make arrests: a member of the police.</rdfs:comment>
        <rdfs:isDefinedBy xml:lang="en">A person whose job is to enforce laws, investigate crimes, and make arrests: a member of the police.</rdfs:isDefinedBy>
        <rdfs:label xml:lang="en">policeAgent</rdfs:label>
    </owl:Class>
    


    <!-- http://localhost:8080/BFiaO/EmergencyAgent#psychologistAgent -->


    <owl:Class rdf:about="http://localhost:8080/BFiaO/EmergencyAgent#psychologistAgent">
        <rdfs:comment xml:lang="en">An expert or specialist in psychology.</rdfs:comment>
        <rdfs:isDefinedBy xml:lang="en">An expert or specialist in psychology.</rdfs:isDefinedBy>
        <rdfs:label xml:lang="en">psychologistAgent</rdfs:label>
    </owl:Class>
    


    <!-- http://localhost:8080/BFiaO/EmergencyAgent#regionalEmergencyAgent -->


    <owl:Class rdf:about="http://localhost:8080/BFiaO/EmergencyAgent#regionalEmergencyAgent">
        <rdfs:comment xml:lang="en">It is an agent contracted by  regional government to work in emergencies like fires, floods, winter emergencies, etc.</rdfs:comment>
        <rdfs:isDefinedBy xml:lang="en">It is an agent contracted by  regional government to work in emergencies like fires, floods, winter emergencies, etc.</rdfs:isDefinedBy>
        <rdfs:label xml:lang="en">regionalEmergencyAgent</rdfs:label>
    </owl:Class>
    


    <!-- http://localhost:8080/BFiaO/EmergencyAgent#signalCorpsAgent -->


    <owl:Class rdf:about="http://localhost:8080/BFiaO/EmergencyAgent#signalCorpsAgent">
        <rdfs:comment xml:lang="en">A soldier who belongs to Signal Corps, which the part of an army in charge of communications.</rdfs:comment>
        <rdfs:isDefinedBy xml:lang="en">A soldier who belongs to Signal Corps, which the part of an army in charge of communications.</rdfs:isDefinedBy>
        <rdfs:label xml:lang="en">signalCorpsAgent</rdfs:label>
    </owl:Class>
    


    <!-- http://localhost:8080/BFiaO/EmergencyAgent#uMEAgent -->


    <owl:Class rdf:about="http://localhost:8080/BFiaO/EmergencyAgent#uMEAgent">
        <rdfs:comment xml:lang="en">A UME Agent is a person with training in different kind of emergencies who belongs to UME (Emergency Military Unit). CBRN is an acronym for Chemical, Biological, Radiological and Nuclear.</rdfs:comment>
        <rdfs:isDefinedBy xml:lang="en">A UME Agent is a person with training in different kind of emergencies who belongs to UME (Emergency Military Unit). CBRN is an acronym for Chemical, Biological, Radiological and Nuclear.</rdfs:isDefinedBy>
        <rdfs:label xml:lang="en">uMEAgent</rdfs:label>
    </owl:Class>
    


    <!-- http://localhost:8080/BFiaO/EmergencyAgent#uMEHelicopterPilotAgent -->


    <owl:Class rdf:about="http://localhost:8080/BFiaO/EmergencyAgent#uMEHelicopterPilotAgent">
        <rdfs:comment xml:lang="en">A person who belong to UME (Emergency Military Unit) and has a license to pilot a helicopter. A pilot is posted to UME Helicopter Unit which is a body of Army Aviation adscribed to UME. It can fly in reconnaissance missions, as post command or dropping water in a fire.</rdfs:comment>
        <rdfs:isDefinedBy xml:lang="en">A military pilot who belong to UME (Emergency Military Unit) and has a license to pilot a helicopter. A pilot is posted to UME Helicopter Unit which is a body of Army Aviation adscribed to UME. It can fly in reconnaissance missions, as post command or dropping water in a fire.</rdfs:isDefinedBy>
        <rdfs:label xml:lang="en">uMEHelicopterPilotAgent</rdfs:label>
    </owl:Class>
    


    <!-- http://localhost:8080/BFiaO/EmergencyAgent#volunteerAgent -->


    <owl:Class rdf:about="http://localhost:8080/BFiaO/EmergencyAgent#volunteerAgent">
        <rdfs:comment xml:lang="en">Volunteer represent citizens that acts individually helping during emergencies.</rdfs:comment>
        <rdfs:isDefinedBy xml:lang="en">Volunteer represent citizens that acts individually helping during emergencies.</rdfs:isDefinedBy>
        <rdfs:label xml:lang="en">volunteerAgent</rdfs:label>
    </owl:Class>
    


    <!-- http://localhost:8080/BFiaO/EmergencyAgent#volunteerAmbulanceDriverAgent -->


    <owl:Class rdf:about="http://localhost:8080/BFiaO/EmergencyAgent#volunteerAmbulanceDriverAgent">
        <rdfs:subClassOf rdf:resource="http://localhost:8080/BFiaO/EmergencyAgent#volunteerAgent"/>
        <rdfs:comment xml:lang="en">A volunteer who has the right license and drives an ambulance.</rdfs:comment>
        <rdfs:isDefinedBy xml:lang="en">A volunteer who has the right license and drives an ambulance.</rdfs:isDefinedBy>
        <rdfs:label xml:lang="en">volunteerAmbulanceDriverAgent</rdfs:label>
    </owl:Class>
    


    <!-- http://localhost:8080/BFiaO/EmergencyAgent#volunteerBusDriverAgent -->


    <owl:Class rdf:about="http://localhost:8080/BFiaO/EmergencyAgent#volunteerBusDriverAgent">
        <rdfs:subClassOf rdf:resource="http://localhost:8080/BFiaO/EmergencyAgent#volunteerAgent"/>
        <rdfs:comment xml:lang="en">A volunteer who is a driver with license to drive a bus.</rdfs:comment>
        <rdfs:isDefinedBy xml:lang="en">A volunteer who is a driver with license to drive a bus.</rdfs:isDefinedBy>
        <rdfs:label xml:lang="en">volunteerBusDriverAgent</rdfs:label>
    </owl:Class>
    


    <!-- http://localhost:8080/BFiaO/EmergencyAgent#volunteerCitizenAgent -->


    <owl:Class rdf:about="http://localhost:8080/BFiaO/EmergencyAgent#volunteerCitizenAgent">
        <rdfs:subClassOf rdf:resource="http://localhost:8080/BFiaO/EmergencyAgent#volunteerAgent"/>
        <rdfs:comment xml:lang="en">A volunteer who voluntarily undertakes or expresses a willingness to undertake a service.</rdfs:comment>
        <rdfs:isDefinedBy xml:lang="en">A volunteer who voluntarily undertakes or expresses a willingness to undertake a service.</rdfs:isDefinedBy>
        <rdfs:label xml:lang="en">volunteerCitizenAgent</rdfs:label>
    </owl:Class>
    


    <!-- http://localhost:8080/BFiaO/EmergencyAgent#volunteerCivilProtectionAgent -->


    <owl:Class rdf:about="http://localhost:8080/BFiaO/EmergencyAgent#volunteerCivilProtectionAgent">
        <rdfs:subClassOf rdf:resource="http://localhost:8080/BFiaO/EmergencyAgent#volunteerAgent"/>
        <rdfs:comment xml:lang="en">Is a volunteer who belongs to Civil Protection.</rdfs:comment>
        <rdfs:isDefinedBy xml:lang="en">Is a volunteer who belongs to Civil Protection.</rdfs:isDefinedBy>
        <rdfs:label xml:lang="en">volunteerCivilProtectionAgent</rdfs:label>
    </owl:Class>
    


    <!-- http://localhost:8080/BFiaO/EmergencyAgent#volunteerGeneralServicesAgent -->


    <owl:Class rdf:about="http://localhost:8080/BFiaO/EmergencyAgent#volunteerGeneralServicesAgent">
        <rdfs:subClassOf rdf:resource="http://localhost:8080/BFiaO/EmergencyAgent#volunteerAgent"/>
        <rdfs:comment xml:lang="en">It defines a volunteer who does not have any specific training and can be used to help in general services like food delivery, food preparation, or cleaning services.</rdfs:comment>
        <rdfs:isDefinedBy xml:lang="en">It defines a volunteer who does not have any specific training and can be used to help in general services like food delivery, food preparation, or cleaning services.</rdfs:isDefinedBy>
        <rdfs:label xml:lang="en">volunteerGeneralServicesAgent</rdfs:label>
    </owl:Class>
    


    <!-- http://localhost:8080/BFiaO/EmergencyAgent#volunteerRedCrossAgent -->


    <owl:Class rdf:about="http://localhost:8080/BFiaO/EmergencyAgent#volunteerRedCrossAgent">
        <rdfs:subClassOf rdf:resource="http://localhost:8080/BFiaO/EmergencyAgent#volunteerAgent"/>
        <rdfs:comment xml:lang="en">A volunteer who belongs to Red Cross Organization. The Red Cross is an international organization that helps people who are suffering, for example as a result of war, floods, or disease.</rdfs:comment>
        <rdfs:isDefinedBy xml:lang="en">A volunteer who belongs to Red Cross Organization. The Red Cross is an international organization that helps people who are suffering, for example as a result of war, floods, or disease.</rdfs:isDefinedBy>
        <rdfs:label xml:lang="en">volunteerRedCrossAgent</rdfs:label>
    </owl:Class>
    


    <!-- http://localhost:8080/BFiaO/EmergencyAgent#volunteerTruckDriverAgent -->


    <owl:Class rdf:about="http://localhost:8080/BFiaO/EmergencyAgent#volunteerTruckDriverAgent">
        <rdfs:subClassOf rdf:resource="http://localhost:8080/BFiaO/EmergencyAgent#volunteerAgent"/>
        <rdfs:comment xml:lang="en">A volunteer who has a driver licence to drive a truck.</rdfs:comment>
        <rdfs:isDefinedBy xml:lang="en">A volunteer who has a driver licence to drive a truck.</rdfs:isDefinedBy>
        <rdfs:label xml:lang="en">volunteerTruckDriverAgent</rdfs:label>
    </owl:Class>
    


    <!-- 
    ///////////////////////////////////////////////////////////////////////////////////////
    //
    // General axioms
    //
    ///////////////////////////////////////////////////////////////////////////////////////
     -->


    <rdf:Description>
        <rdf:type rdf:resource="http://www.w3.org/2002/07/owl#AllDisjointClasses"/>
        <owl:members rdf:parseType="Collection">
            <rdf:Description rdf:about="http://localhost:8080/BFiaO/EmergencyAgent#armedForcesAgent"/>
            <rdf:Description rdf:about="http://localhost:8080/BFiaO/EmergencyAgent#armedForcesFireExtinguisherPlanePilotAgent"/>
            <rdf:Description rdf:about="http://localhost:8080/BFiaO/EmergencyAgent#armedForcesHelicopterPilotAgent"/>
            <rdf:Description rdf:about="http://localhost:8080/BFiaO/EmergencyAgent#bRIFAgent"/>
            <rdf:Description rdf:about="http://localhost:8080/BFiaO/EmergencyAgent#cBRNAgent"/>
            <rdf:Description rdf:about="http://localhost:8080/BFiaO/EmergencyAgent#cBRNArmedForcesAgent"/>
            <rdf:Description rdf:about="http://localhost:8080/BFiaO/EmergencyAgent#cBRNUMEAgent"/>
            <rdf:Description rdf:about="http://localhost:8080/BFiaO/EmergencyAgent#doctorAgent"/>
            <rdf:Description rdf:about="http://localhost:8080/BFiaO/EmergencyAgent#fireBrigadeAgent"/>
            <rdf:Description rdf:about="http://localhost:8080/BFiaO/EmergencyAgent#guardiaCivilAgent"/>
            <rdf:Description rdf:about="http://localhost:8080/BFiaO/EmergencyAgent#healthCareWorkerAgent"/>
            <rdf:Description rdf:about="http://localhost:8080/BFiaO/EmergencyAgent#policeAgent"/>
            <rdf:Description rdf:about="http://localhost:8080/BFiaO/EmergencyAgent#psychologistAgent"/>
            <rdf:Description rdf:about="http://localhost:8080/BFiaO/EmergencyAgent#regionalEmergencyAgent"/>
            <rdf:Description rdf:about="http://localhost:8080/BFiaO/EmergencyAgent#signalCorpsAgent"/>
            <rdf:Description rdf:about="http://localhost:8080/BFiaO/EmergencyAgent#uMEAgent"/>
            <rdf:Description rdf:about="http://localhost:8080/BFiaO/EmergencyAgent#uMEHelicopterPilotAgent"/>
            <rdf:Description rdf:about="http://localhost:8080/BFiaO/EmergencyAgent#volunteerAgent"/>
        </owl:members>
    </rdf:Description>
    <rdf:Description>
        <rdf:type rdf:resource="http://www.w3.org/2002/07/owl#AllDisjointClasses"/>
        <owl:members rdf:parseType="Collection">
            <rdf:Description rdf:about="http://localhost:8080/BFiaO/EmergencyAgent#volunteerAmbulanceDriverAgent"/>
            <rdf:Description rdf:about="http://localhost:8080/BFiaO/EmergencyAgent#volunteerBusDriverAgent"/>
            <rdf:Description rdf:about="http://localhost:8080/BFiaO/EmergencyAgent#volunteerCitizenAgent"/>
            <rdf:Description rdf:about="http://localhost:8080/BFiaO/EmergencyAgent#volunteerCivilProtectionAgent"/>
            <rdf:Description rdf:about="http://localhost:8080/BFiaO/EmergencyAgent#volunteerGeneralServicesAgent"/>
            <rdf:Description rdf:about="http://localhost:8080/BFiaO/EmergencyAgent#volunteerRedCrossAgent"/>
            <rdf:Description rdf:about="http://localhost:8080/BFiaO/EmergencyAgent#volunteerTruckDriverAgent"/>
        </owl:members>
    </rdf:Description>
</rdf:RDF>



<!-- Generated by the OWL API (version 5.1.18) https://github.com/owlcs/owlapi/ -->


