@prefix : <http://localhost:8080/BFiaO/EmergencyAgent#> .
@prefix owl: <http://www.w3.org/2002/07/owl#> .
@prefix rdf: <http://www.w3.org/1999/02/22-rdf-syntax-ns#> .
@prefix xml: <http://www.w3.org/XML/1998/namespace> .
@prefix xsd: <http://www.w3.org/2001/XMLSchema#> .
@prefix rdfs: <http://www.w3.org/2000/01/rdf-schema#> .
@base <http://localhost:8080/BFiaO/EmergencyAgent#> .

<http://localhost:8080/BFiaO/EmergencyAgent> rdf:type owl:Ontology ;
                                              <http://creativecommons.org/ns#license> <https://spdx.org/licenses/MIT.html> ;
                                              :content_license """The MIT License (MIT)

Copyright (c) 2022 Leopoldo Santos Santos of Strategic Sector

Permission is hereby granted, free of charge, to any person obtaining a copy
of this software and associated documentation files (the \"Software\"), to deal
in the Software without restriction, including without limitation the rights
to use, copy, modify, merge, publish, distribute, sublicense, and/or sell
copies of the Software, and to permit persons to whom the Software is
furnished to do so, subject to the following conditions:

The above copyright notice and this permission notice shall be included in
all copies or substantial portions of the Software.

THE SOFTWARE IS PROVIDED \"AS IS\", WITHOUT WARRANTY OF ANY KIND, EXPRESS OR
IMPLIED, INCLUDING BUT NOT LIMITED TO THE WARRANTIES OF MERCHANTABILITY,
FITNESS FOR A PARTICULAR PURPOSE AND NONINFRINGEMENT. IN NO EVENT SHALL THE
AUTHORS OR COPYRIGHT HOLDERS BE LIABLE FOR ANY CLAIM, DAMAGES OR OTHER
LIABILITY, WHETHER IN AN ACTION OF CONTRACT, TORT OR OTHERWISE, ARISING FROM,
OUT OF OR IN CONNECTION WITH THE SOFTWARE OR THE USE OR OTHER DEALINGS IN
THE SOFTWARE."""@en ;
                                              <http://purl.org/dc/elements/1.1/creator> "Leopoldo Santos Santos"@en ;
                                              rdfs:comment "This ontology is designed to identify the emergency agents who can act in an emergency situation."@en ;
                                              rdfs:label "Emergency Agent" ;
                                              owl:versionInfo "Version 1.0"@en .

#################################################################
#    Annotation properties
#################################################################

###  http://creativecommons.org/ns#license
<http://creativecommons.org/ns#license> rdf:type owl:AnnotationProperty .


###  http://localhost:8080/BFiaO/EmergencyAgent#content_license
:content_license rdf:type owl:AnnotationProperty .


###  http://purl.org/dc/elements/1.1/creator
<http://purl.org/dc/elements/1.1/creator> rdf:type owl:AnnotationProperty .


#################################################################
#    Data properties
#################################################################

###  http://localhost:8080/BFiaO/EmergencyAgent#AgentDeployedGeolocation
:AgentDeployedGeolocation rdf:type owl:DatatypeProperty ;
                          rdfs:comment "This atribute has the geolacation of the agent."@en ;
                          rdfs:isDefinedBy "This atribute has the geolacation of the agent."@en ;
                          rdfs:label "AgentDeployedGeolocation"@en .


###  http://localhost:8080/BFiaO/EmergencyAgent#AgentEndUseTransctionTime
:AgentEndUseTransctionTime rdf:type owl:DatatypeProperty ;
                           rdfs:comment "It identifies the transaction time for the completion time of use of an artifact by an agent."@en ;
                           rdfs:isDefinedBy "It identifies the transaction time for the completion time of use of an artifact by an agent."@en ;
                           rdfs:label "AgentEndUseTransctionTime"@en .


###  http://localhost:8080/BFiaO/EmergencyAgent#AgentEndUseValidTime
:AgentEndUseValidTime rdf:type owl:DatatypeProperty ;
                      rdfs:comment "It identifies the completion time of use of an artifact by an agent."@en ;
                      rdfs:isDefinedBy "It identifies the completion time of use of an artifact by an agent."@en ;
                      rdfs:label "AgentEndUseValidTime"@en .


###  http://localhost:8080/BFiaO/EmergencyAgent#AgentName
:AgentName rdf:type owl:DatatypeProperty ;
           rdfs:comment "It identifes the name of an agent."@en ;
           rdfs:isDefinedBy "It identifes the name of an agent."@en ;
           rdfs:label "AgentName"@en .


###  http://localhost:8080/BFiaO/EmergencyAgent#AgentPhone
:AgentPhone rdf:type owl:DatatypeProperty ;
            rdfs:comment "It identifies the phone of the agent."@en ;
            rdfs:isDefinedBy "It identifies the phone of the agent."@en ;
            rdfs:label "AgentPhone"@en .


###  http://localhost:8080/BFiaO/EmergencyAgent#AgentRank
:AgentRank rdf:type owl:DatatypeProperty ;
           rdfs:comment "It identifies the rank of an agent."@en ;
           rdfs:isDefinedBy "It identifies the rank of an agent."@en ;
           rdfs:label "AgentRank"@en .


###  http://localhost:8080/BFiaO/EmergencyAgent#AgentStartUseTransactionTime
:AgentStartUseTransactionTime rdf:type owl:DatatypeProperty ;
                              rdfs:comment "It identifies the transaction tiem for start time of use of an artifact by an agent."@en ;
                              rdfs:isDefinedBy "It identifies the transaction tiem for start time of use of an artifact by an agent."@en ;
                              rdfs:label "AgentStartUseTransactionTime"@en .


###  http://localhost:8080/BFiaO/EmergencyAgent#AgentStartUseValidTime
:AgentStartUseValidTime rdf:type owl:DatatypeProperty ;
                        rdfs:subPropertyOf owl:topDataProperty ;
                        rdfs:comment "It identifies the start time of use of an artifact by an agent."@en ;
                        rdfs:isDefinedBy "It identifies the start time of use of an artifact by an agent."@en ;
                        rdfs:label "AgentStartUseValidTime"@en .


###  http://localhost:8080/BFiaO/EmergencyAgent#AgentUnitID
:AgentUnitID rdf:type owl:DatatypeProperty ;
             rdfs:comment "It identifies the identification code for the Unit."@en ;
             rdfs:isDefinedBy "It identifies the identification code for the Unit."@en ;
             rdfs:label "AgentUnitID"@en .


#################################################################
#    Classes
#################################################################

###  http://localhost:8080/BFiaO/EmergencyAgent#armedForcesAgent
:armedForcesAgent rdf:type owl:Class ;
                  rdfs:comment "It is a person who belongs to Armed Forces."@en ;
                  rdfs:isDefinedBy "It is a person who belongs to Armed Forces."@en ;
                  rdfs:label "armedForcesAgent"@en .


###  http://localhost:8080/BFiaO/EmergencyAgent#armedForcesFireExtinguisherPlanePilotAgent
:armedForcesFireExtinguisherPlanePilotAgent rdf:type owl:Class ;
                                            rdfs:comment "A military pilot who has a license to pilot aircraft and specialized in piloting firefighting aircraft."@en ;
                                            rdfs:isDefinedBy "A military pilot who has a license to pilot aircraft and specialized in piloting firefighting aircraft."@en ;
                                            rdfs:label "armedForcesFireExtinguisherPlanePilotAgent"@en .


###  http://localhost:8080/BFiaO/EmergencyAgent#armedForcesHelicopterPilotAgent
:armedForcesHelicopterPilotAgent rdf:type owl:Class ;
                                 rdfs:comment "A military pilot who belong to Armed Forces and has a license to pilot a helicopter."@en ;
                                 rdfs:isDefinedBy "A military pilot who belong to Armed Forces and has a license to pilot a helicopter."@en ;
                                 rdfs:label "armedForcesHelicopterPilotAgent"@en .


###  http://localhost:8080/BFiaO/EmergencyAgent#bRIFAgent
:bRIFAgent rdf:type owl:Class ;
           rdfs:comment "It is an agent who belongs to a BRIF."@en ;
           rdfs:isDefinedBy "It is an agent who belongs to a BRIF."@en ;
           rdfs:label "bRIFAgent"@en .


###  http://localhost:8080/BFiaO/EmergencyAgent#cBRNAgent
:cBRNAgent rdf:type owl:Class ;
           rdfs:comment "A CBRN Agent is a person with training in CBRN. CBRN is an acronym for Chemical, Biological, Radiological and Nuclear."@en ;
           rdfs:isDefinedBy "A CBRN Agent is a person with training in CBRN. CBRN is an acronym for Chemical, Biological, Radiological and Nuclear."@en ;
           rdfs:label "cBRNAgent"@en .


###  http://localhost:8080/BFiaO/EmergencyAgent#cBRNArmedForcesAgent
:cBRNArmedForcesAgent rdf:type owl:Class ;
                      rdfs:comment "A CBRN Armed Forces Agent is a person with training in CBRN who belongs to Armed Forces. CBRN is an acronym for Chemical, Biological, Radiological and Nuclear."@en ;
                      rdfs:isDefinedBy "A CBRN Armed Forces Agent is a person with training in CBRN who belongs to Armed Forces. CBRN is an acronym for Chemical, Biological, Radiological and Nuclear."@en ;
                      rdfs:label "cBRNArmedForcesAgent"@en .


###  http://localhost:8080/BFiaO/EmergencyAgent#cBRNUMEAgent
:cBRNUMEAgent rdf:type owl:Class ;
              rdfs:comment "A UME CBRN Agent is a person with training in CBRN who belongs to UME (Emergency Military Unit). CBRN is an acronym for Chemical, Biological, Radiological and Nuclear."@en ;
              rdfs:isDefinedBy "A UME CBRN Agent is a person with training in CBRN who belongs to UME (Emergency Military Unit). CBRN is an acronym for Chemical, Biological, Radiological and Nuclear."@en ;
              rdfs:label "cBRNUMEAgent"@en .


###  http://localhost:8080/BFiaO/EmergencyAgent#doctorAgent
:doctorAgent rdf:type owl:Class ;
             rdfs:comment "A person with a medical degree whose job is to treat people who are ill or hurt and who belongs to any kind of Units working in the Emergency."@en ;
             rdfs:isDefinedBy "A person with a medical degree whose job is to treat people who are ill or hurt and who belongs to any kind of Units working in the Emergency."@en ;
             rdfs:label "doctorAgent"@en .


###  http://localhost:8080/BFiaO/EmergencyAgent#fireBrigadeAgent
:fireBrigadeAgent rdf:type owl:Class ;
                  rdfs:comment "A Fire Brigade Agent is a person with training in fire fighting and works in this field."@en ;
                  rdfs:isDefinedBy "A Fire Brigade Agent is a person with training in fire fighting and works in this field."@en ;
                  rdfs:label "fireBrigadeAgent"@en .


###  http://localhost:8080/BFiaO/EmergencyAgent#guardiaCivilAgent
:guardiaCivilAgent rdf:type owl:Class ;
                   rdfs:comment "Is a person who belongs to Guardia Civil, which is a law enforcement force, a gendarmerie corps with a military nature with a permanent vocation for services."@en ;
                   rdfs:isDefinedBy "Is a person who belongs to Guardia Civil, which is a law enforcement force, a gendarmerie corps with a military nature with a permanent vocation for services."@en ;
                   rdfs:label "guardiaCivilAgent"@en .


###  http://localhost:8080/BFiaO/EmergencyAgent#healthCareWorkerAgent
:healthCareWorkerAgent rdf:type owl:Class ;
                       rdfs:comment "A healthcare worker is anyone who works in a healthcare or social care setting, including healthcare students on clinical placement, frontline healthcare workers and other healthcare workers not in direct patient contact."@en ;
                       rdfs:isDefinedBy "A healthcare worker is anyone who works in a healthcare or social care setting, including healthcare students on clinical placement, frontline healthcare workers and other healthcare workers not in direct patient contact."@en ;
                       rdfs:label "healthCareWorkerAgent"@en .


###  http://localhost:8080/BFiaO/EmergencyAgent#policeAgent
:policeAgent rdf:type owl:Class ;
             rdfs:comment "A person whose job is to enforce laws, investigate crimes, and make arrests: a member of the police."@en ;
             rdfs:isDefinedBy "A person whose job is to enforce laws, investigate crimes, and make arrests: a member of the police."@en ;
             rdfs:label "policeAgent"@en .


###  http://localhost:8080/BFiaO/EmergencyAgent#psychologistAgent
:psychologistAgent rdf:type owl:Class ;
                   rdfs:comment "An expert or specialist in psychology."@en ;
                   rdfs:isDefinedBy "An expert or specialist in psychology."@en ;
                   rdfs:label "psychologistAgent"@en .


###  http://localhost:8080/BFiaO/EmergencyAgent#regionalEmergencyAgent
:regionalEmergencyAgent rdf:type owl:Class ;
                        rdfs:comment "It is an agent contracted by  regional government to work in emergencies like fires, floods, winter emergencies, etc."@en ;
                        rdfs:isDefinedBy "It is an agent contracted by  regional government to work in emergencies like fires, floods, winter emergencies, etc."@en ;
                        rdfs:label "regionalEmergencyAgent"@en .


###  http://localhost:8080/BFiaO/EmergencyAgent#signalCorpsAgent
:signalCorpsAgent rdf:type owl:Class ;
                  rdfs:comment "A soldier who belongs to Signal Corps, which the part of an army in charge of communications."@en ;
                  rdfs:isDefinedBy "A soldier who belongs to Signal Corps, which the part of an army in charge of communications."@en ;
                  rdfs:label "signalCorpsAgent"@en .


###  http://localhost:8080/BFiaO/EmergencyAgent#uMEAgent
:uMEAgent rdf:type owl:Class ;
          rdfs:comment "A UME Agent is a person with training in different kind of emergencies who belongs to UME (Emergency Military Unit). CBRN is an acronym for Chemical, Biological, Radiological and Nuclear."@en ;
          rdfs:isDefinedBy "A UME Agent is a person with training in different kind of emergencies who belongs to UME (Emergency Military Unit). CBRN is an acronym for Chemical, Biological, Radiological and Nuclear."@en ;
          rdfs:label "uMEAgent"@en .


###  http://localhost:8080/BFiaO/EmergencyAgent#uMEHelicopterPilotAgent
:uMEHelicopterPilotAgent rdf:type owl:Class ;
                         rdfs:comment "A person who belong to UME (Emergency Military Unit) and has a license to pilot a helicopter. A pilot is posted to UME Helicopter Unit which is a body of Army Aviation adscribed to UME. It can fly in reconnaissance missions, as post command or dropping water in a fire."@en ;
                         rdfs:isDefinedBy "A military pilot who belong to UME (Emergency Military Unit) and has a license to pilot a helicopter. A pilot is posted to UME Helicopter Unit which is a body of Army Aviation adscribed to UME. It can fly in reconnaissance missions, as post command or dropping water in a fire."@en ;
                         rdfs:label "uMEHelicopterPilotAgent"@en .


###  http://localhost:8080/BFiaO/EmergencyAgent#volunteerAgent
:volunteerAgent rdf:type owl:Class ;
                rdfs:comment "Volunteer represent citizens that acts individually helping during emergencies."@en ;
                rdfs:isDefinedBy "Volunteer represent citizens that acts individually helping during emergencies."@en ;
                rdfs:label "volunteerAgent"@en .


###  http://localhost:8080/BFiaO/EmergencyAgent#volunteerAmbulanceDriverAgent
:volunteerAmbulanceDriverAgent rdf:type owl:Class ;
                               rdfs:subClassOf :volunteerAgent ;
                               rdfs:comment "A volunteer who has the right license and drives an ambulance."@en ;
                               rdfs:isDefinedBy "A volunteer who has the right license and drives an ambulance."@en ;
                               rdfs:label "volunteerAmbulanceDriverAgent"@en .


###  http://localhost:8080/BFiaO/EmergencyAgent#volunteerBusDriverAgent
:volunteerBusDriverAgent rdf:type owl:Class ;
                         rdfs:subClassOf :volunteerAgent ;
                         rdfs:comment "A volunteer who is a driver with license to drive a bus."@en ;
                         rdfs:isDefinedBy "A volunteer who is a driver with license to drive a bus."@en ;
                         rdfs:label "volunteerBusDriverAgent"@en .


###  http://localhost:8080/BFiaO/EmergencyAgent#volunteerCitizenAgent
:volunteerCitizenAgent rdf:type owl:Class ;
                       rdfs:subClassOf :volunteerAgent ;
                       rdfs:comment "A volunteer who voluntarily undertakes or expresses a willingness to undertake a service."@en ;
                       rdfs:isDefinedBy "A volunteer who voluntarily undertakes or expresses a willingness to undertake a service."@en ;
                       rdfs:label "volunteerCitizenAgent"@en .


###  http://localhost:8080/BFiaO/EmergencyAgent#volunteerCivilProtectionAgent
:volunteerCivilProtectionAgent rdf:type owl:Class ;
                               rdfs:subClassOf :volunteerAgent ;
                               rdfs:comment "Is a volunteer who belongs to Civil Protection."@en ;
                               rdfs:isDefinedBy "Is a volunteer who belongs to Civil Protection."@en ;
                               rdfs:label "volunteerCivilProtectionAgent"@en .


###  http://localhost:8080/BFiaO/EmergencyAgent#volunteerGeneralServicesAgent
:volunteerGeneralServicesAgent rdf:type owl:Class ;
                               rdfs:subClassOf :volunteerAgent ;
                               rdfs:comment "It defines a volunteer who does not have any specific training and can be used to help in general services like food delivery, food preparation, or cleaning services."@en ;
                               rdfs:isDefinedBy "It defines a volunteer who does not have any specific training and can be used to help in general services like food delivery, food preparation, or cleaning services."@en ;
                               rdfs:label "volunteerGeneralServicesAgent"@en .


###  http://localhost:8080/BFiaO/EmergencyAgent#volunteerRedCrossAgent
:volunteerRedCrossAgent rdf:type owl:Class ;
                        rdfs:subClassOf :volunteerAgent ;
                        rdfs:comment "A volunteer who belongs to Red Cross Organization. The Red Cross is an international organization that helps people who are suffering, for example as a result of war, floods, or disease."@en ;
                        rdfs:isDefinedBy "A volunteer who belongs to Red Cross Organization. The Red Cross is an international organization that helps people who are suffering, for example as a result of war, floods, or disease."@en ;
                        rdfs:label "volunteerRedCrossAgent"@en .


###  http://localhost:8080/BFiaO/EmergencyAgent#volunteerTruckDriverAgent
:volunteerTruckDriverAgent rdf:type owl:Class ;
                           rdfs:subClassOf :volunteerAgent ;
                           rdfs:comment "A volunteer who has a driver licence to drive a truck."@en ;
                           rdfs:isDefinedBy "A volunteer who has a driver licence to drive a truck."@en ;
                           rdfs:label "volunteerTruckDriverAgent"@en .


#################################################################
#    General axioms
#################################################################

[ rdf:type owl:AllDisjointClasses ;
  owl:members ( :armedForcesAgent
                :armedForcesFireExtinguisherPlanePilotAgent
                :armedForcesHelicopterPilotAgent
                :bRIFAgent
                :cBRNAgent
                :cBRNArmedForcesAgent
                :cBRNUMEAgent
                :doctorAgent
                :fireBrigadeAgent
                :guardiaCivilAgent
                :healthCareWorkerAgent
                :policeAgent
                :psychologistAgent
                :regionalEmergencyAgent
                :signalCorpsAgent
                :uMEAgent
                :uMEHelicopterPilotAgent
                :volunteerAgent
              )
] .


[ rdf:type owl:AllDisjointClasses ;
  owl:members ( :volunteerAmbulanceDriverAgent
                :volunteerBusDriverAgent
                :volunteerCitizenAgent
                :volunteerCivilProtectionAgent
                :volunteerGeneralServicesAgent
                :volunteerRedCrossAgent
                :volunteerTruckDriverAgent
              )
] .


###  Generated by the OWL API (version 5.1.18) https://github.com/owlcs/owlapi/
